msi: Restructure IOAPIC, MSI interrupts for x86, fix up ARM proofs for new API

spec/abstract/Invocations_A.thy
@@ -52,7 +52,6 @@ datatype irq_handler_invocation =
     ACKIrq irq
   | SetIRQHandler irq cap cslot_ptr
   | ClearIRQHandler irq
-  | SetMode irq bool bool
 
 datatype invocation =
     InvokeUntyped untyped_invocation
