proof/drefine/Syscall_DR.thy
@@ -326,7 +326,6 @@ lemma decode_invocation_irqhandlercap_corres:
   apply (clarsimp simp: throw_opt_def get_irq_handler_intent_def split: option.splits)
   apply (rule conjI)
    apply (auto simp: decode_irq_handler_invocation_def transform_intent_def
-                     transform_intent_irq_set_mode_def 
           split del: split_if 
               split: invocation_label.splits cdl_intent.splits list.splits)[1]
   apply clarsimp
@@ -441,7 +440,7 @@ lemma transform_intent_irq_handler_None:
   apply (clarsimp simp:Decode_A.decode_invocation_def)
   apply (wp)
     apply (clarsimp simp:decode_irq_handler_invocation_def|rule conjI)+
-      apply (clarsimp simp:transform_intent_def transform_intent_irq_set_mode_def split: list.splits)+
+      apply (clarsimp simp:transform_intent_def split: list.splits)+
     apply (clarsimp simp:transform_intent_def |rule conjI | wp)+
 done
 
