spec/capDL/Intents_D.thy
@@ -127,8 +127,6 @@ datatype cdl_irq_handler_intent =
  |  IrqHandlerSetEndpointIntent
     (* Clear: (target) *)
  |  IrqHandlerClearIntent
-    (* SetMode: (target) trig pol *)
- |  IrqHandlerSetModeIntent bool bool 
 
 datatype cdl_irq_control_intent =
     (* IssueIrqHandler: (target), irq, (root), index, depth *)
